---
tags: concept
---
# Latex
$$f^{-1}(x) = \frac{x-1}{-4} $$
***


$$(n+1)^{2} - n^2 = n + (n+1) $$
$$ n^2 + 2n + 1 - n^2 = 2n + 1 $$
$$ 2n + 1 = 2n + 1 $$
***


$$\cos^2x + \sin^2x = 1$$
***
$$\frac{x+1}{2x-1}=\frac{x-3}{2x+1}$$$$\left(x+1\right)\left(2x+1\right)=\left(x-3\right)\left(2x-1\right)$$$$2x^2+x+2x+1=2x^2-x-6x+3$$
$$3x+1=-7x+3$$
$$10x=2$$
$$x=2/10$$

***
$$3x+5y=5$$
$$2x+y=1$$
$$3x=5-5y$$
$$x=\frac{5-5y}{3}$$
$$2\left(\frac{5-5y}{3}\right)+y=1$$
$$\frac{10-10y}{3}+y=1$$
$$10-10y+3y=3$$
$$-7y=-7$$
$$y=1$$
$$3x+5=5$$
$$3x=0$$
$$x=0$$
***
$$\sigma=\sqrt{\frac{\sum\left(x-\mu\right)^2}n}$$
$$\sigma=\sqrt{\frac{\sum\left(x^2-2x\mu+\mu^2\right)}n}$$
$$\sigma=\sqrt{\frac{\sum x^2-\sum 2x\mu+\sum\mu^2}{n}}$$
$$\sigma=\sqrt{\frac{\sum x^2}{n}-\frac{\sum 2x\mu}{n}+\frac{\sum\mu^2}{n}}$$
$$\sigma=\sqrt{\frac{\sum x^2}{n}-2\mu\frac{\sum x}{n}+\frac{\sum\mu^2}{n}}$$
$$\sigma=\sqrt{\frac{\sum x^2}{n}-2\mu\mu+\mu^2}$$
$$\sigma=\sqrt{\frac{\sum x^2}{n}-2\mu^2+\mu^2}$$
$$\sigma=\sqrt{\frac{\sum x^2}{n}-\mu^2}$$
$$\sigma=\sqrt{\frac{\sum x^2}{n}-\left(\frac{\sum x}{n}\right)^2}$$
***
$$n\frac{(n+3)\frac{(n+2)\frac{(n+1)}{2}}{3}}{8}$$
 
 
<!--ID: 1664475094981-->




***
$$x\left(\frac{5}{2}\right)$$
$$x\left(\frac{5}{2}\right)$$
<!--ID: 1664475647499-->


$$x\left(\frac{5}{2}\right)$$
<!--ID: 1664475094984-->



$$x\left(\frac{5}{2}\right)$$
$$x\left(\frac{5}{2}\right)$$
<!--ID: 1664475647505-->


$$\cdot$$
<!--ID: 1664475094986-->


***
$$\bar{v}=\frac{\Delta x}{t}=\frac{v+v_{0}}{2}$$
$$a=\frac{\Delta v}{t}=\frac{v-v_{0}}{t}$$
***
$$\lim_{x\to 3}\frac{x-3}{x^{2}-9}$$
$$\lim_{x\to 3}\frac{(x-3)}{(x-3)(x+3)}$$
$$\lim_{x\to 3}\frac{1}{x+3}$$
$$\frac{1}{6}$$
```python
a = False
if a:
	print('hello world')
else:
	print('no')
```
<!--ID: 1664475647511-->
<!--ID: 1664475094989-->

---
$$f\left(x\right)=ln\left(x-1\right)+ln\left(3\right)$$
$$y=ln\left(x-1\right)+ln\left(3\right)$$
$$y=ln\left(3x-3\right)$$
$$y=log_e\left(3x-3\right)$$
$$e^y=3x-3$$
$$e^y+3=3x$$
$$\frac{1}{3}e^y+1=x$$
$$f^{-1}(x)=\frac{1}{3}e^x+1$$
